StringDb might be done

platform/tests/StringDb.v
@@ -26,10 +26,13 @@ Module Type TREE.
     -> (Ex t1, Ex t2, Ex i, Ex c, Ex p1, Ex p2, [| t = Node t1 t2 |] * (p ==*> i, c, p1, p2)
         * tree'' b t1 p1 c * tree' b t2 p2) ===> tree' b t p.
 
+  Axiom tree'_weaken : forall b b', b %<= b'
+    -> forall t p, tree' b t p ===> tree' b' t p.
+
   Axiom tree''_zero_fwd : forall b t p (c : W), c = 0
-    -> tree'' b t p c ===> [| p %in b |].
+    -> tree'' b t p c ===> [| p %in b |] * [| t = Leaf |].
   Axiom tree''_zero_bwd : forall b t p (c : W), c = 0
-    -> [| p %in b |] ===> tree'' b t p c.
+    -> [| p %in b |] * [| t = Leaf |] ===> tree'' b t p c.
 
   Axiom tree''_nonzero_fwd : forall b t p (c : W), c <> 0
     -> tree'' b t p c ===> tree' b t p.
@@ -44,12 +47,12 @@ Module Tree : TREE.
     match t with
       | Leaf => [| p = 0 |]
       | Node t1 t2 => [| p <> 0 |] * Ex i, Ex c, Ex p1, Ex p2, (p ==*> i, c, p1, p2)
-        * (if weq c $0 then [| p1 %in b |] else tree' b t1 p1) * tree' b t2 p2
+        * (if weq c $0 then [| p1 %in b |] * [| t1 = Leaf |] else tree' b t1 p1) * tree' b t2 p2
     end.
 
   Definition tree'' (b : bag) (t : shape) (p c : W) : HProp :=
     if weq c $0
-      then [| p %in b |]
+      then [| p %in b |] * [| t = Leaf |]
       else tree' b t p.
 
   Definition tree (b : bag) (p : W) : HProp := Ex t, Ex p', Ex junk, (p ==*> p', junk) * tree' b t p'.
@@ -66,7 +69,7 @@ Module Tree : TREE.
     match goal with
       | [ |- context C[(Ex i : W, Ex c : W, Ex p1 : W, Ex p2 : W,
         ?p =*> i * ((?p ^+ $4) =*> c * ((?p ^+ $8) =*> p1 * (?p ^+ $12) =*> p2))
-        * (if weq c $0 then [| p1 %in ?b |] else tree' ?b ?t1 p1) * tree' ?b ?t2 p2)%Sep] ] =>
+        * (if weq c $0 then [| p1 %in ?b |] * [| ?t1 = Leaf |] else tree' ?b ?t1 p1) * tree' ?b ?t2 p2)%Sep] ] =>
       let G := context C[(Ex i : W, Ex c : W, Ex p1 : W, Ex p2 : W,
         p =*> i * ((p ^+ $4) =*> c * ((p ^+ $8) =*> p1 * (p ^+ $12) =*> p2))
         * tree'' b t1 p1 c * tree' b t2 p2)%Sep] in
@@ -98,15 +101,22 @@ Module Tree : TREE.
       end.
   Qed.
 
+  Theorem tree'_weaken : forall b b', b %<= b'
+    -> forall t p, tree' b t p ===> tree' b' t p.
+    induction t; simpl; intros; repeat normalize; sepLemma;
+      apply himp_star_frame; auto;
+        unfold tree''; destruct (weq x1 $0); auto; sepLemma; eauto using incl_mem.
+  Qed.
+
   Transparent natToWord.
 
   Theorem tree''_zero_fwd : forall b t p (c : W), c = 0
-    -> tree'' b t p c ===> [| p %in b |].
+    -> tree'' b t p c ===> [| p %in b |] * [| t = Leaf |].
     unfold tree''; intros; subst; sepLemma.
   Qed.
 
   Theorem tree''_zero_bwd : forall b t p (c : W), c = 0
-    -> [| p %in b |] ===> tree'' b t p c.
+    -> [| p %in b |] * [| t = Leaf |] ===> tree'' b t p c.
     unfold tree''; intros; subst; sepLemma.
   Qed.
 
@@ -119,6 +129,7 @@ Module Tree : TREE.
     -> tree' b t p ===> tree'' b t p c.
     unfold tree''; intros; destruct (weq c $0); sepLemma.
   Qed.
+
 End Tree.
 
 Import Tree.
@@ -138,12 +149,17 @@ Definition newS := SPEC reserving 8
   PRE[_] mallocHeap 0
   POST[R] tree empty R * mallocHeap 0.
 
-Definition lookupS := SPEC("t", "key", "keyLen") reserving 49
+Definition lookupS := SPEC("t", "key", "keyLen") reserving 2
   Al b,
   PRE[V] tree b (V "t") * V "key" =?>8 wordToNat (V "keyLen")
   POST[R] [| R = 0 \/ R %in b |] * tree b (V "t") * V "key" =?>8 wordToNat (V "keyLen").
 
-Definition m := bimport [[ "malloc"!"malloc" @ [mallocS] ]]
+Definition insertS := SPEC("t", "key", "keyLen", "value") reserving 13
+  Al b,
+  PRE[V] tree b (V "t") * V "key" =?>8 wordToNat (V "keyLen") * mallocHeap 0
+  POST[_] tree (b %+ V "value") (V "t") * V "key" =?>8 wordToNat (V "keyLen") * mallocHeap 0.
+
+Definition m := bimport [[ "malloc"!"malloc" @ [mallocS], "sys"!"abort" @ [abortS] ]]
   bmodule "stringdb" {{
     bfunction "new"("r") [newS]
       "r" <-- Call "malloc"!"malloc"(0, 2)
@@ -204,6 +220,125 @@ Definition m := bimport [[ "malloc"!"malloc" @ [mallocS] ]]
       };;
 
       Return 0
+    end with bfunction "insert"("t", "key", "keyLen", "value", "p", "pos", "i", "c", "c2", "matched") [insertS]
+      "p" <-* "t";;
+      "pos" <- 0;;
+
+      [Al b, Al t,
+        PRE[V] V "t" =*> V "p" * tree' b t (V "p") * V "key" =?>8 wordToNat (V "keyLen") * mallocHeap 0
+        POST[_] Ex p, Ex t', V "t" =*> p * tree' (b %+ V "value") t' p * V "key" =?>8 wordToNat (V "keyLen")
+          * mallocHeap 0]
+      While (0 = 0) {
+        If ("pos" < "keyLen") {
+          (* We are in the phase of matching characters in key. *)
+
+          (* Read current character from key. *)
+          Note [debufferize];;
+
+          Assert [Al b, Al t, Al bs,
+            PRE[V] V "t" =*> V "p" * tree' b t (V "p") * array8 bs (V "key") * mallocHeap 0
+              * [| length bs = wordToNat (V "keyLen") |] * [| (V "pos" < natToW (length bs))%word |]
+            POST[_] Ex p, Ex t', V "t" =*> p * tree' (b %+ V "value") t' p
+              * V "key" =?>8 wordToNat (V "keyLen") * mallocHeap 0];;
+
+          "c2" <- "key" + "pos";;
+          "c2" <-*8 "c2";;
+
+          Note [debufferize];;
+
+          Assert [Al b, Al t,
+            PRE[V] V "t" =*> V "p" * tree' b t (V "p")
+              * V "key" =?>8 wordToNat (V "keyLen") * mallocHeap 0
+            POST[_] Ex p, Ex t', V "t" =*> p * tree' (b %+ V "value") t' p
+              * V "key" =?>8 wordToNat (V "keyLen") * mallocHeap 0];;
+
+          If ("p" = 0) {
+            "matched" <- 0
+          } else {
+            "i" <-* "p";;
+            If ("i" = "pos") {
+              "matched" <- 1
+            } else {
+              "matched" <- 0
+            }
+          };;
+
+          If ("matched" = 1) {
+            Assert [Al b, Al i, Al c, Al p1, Al p2, Al t1, Al t2, 
+              PRE[V] [| V "p" <> 0 |] * V "t" =*> V "p" * (V "p" ==*> i, c, p1, p2)
+                * tree'' b t1 p1 c * tree' b t2 p2
+                * V "key" =?>8 wordToNat (V "keyLen") * mallocHeap 0
+              POST[_] Ex p, Ex t', V "t" =*> p * tree' (b %+ V "value") t' p
+                * V "key" =?>8 wordToNat (V "keyLen") * mallocHeap 0];;
+
+            (* The next test in the tree matches the character we are focusing on. *)
+            "c" <-* "p"+4;;
+
+            If ("c" = 0) {
+              (* This is a length test that fails for us. *)
+              "t" <- "p"+12
+            } else {
+              If ("c2" = "c") {
+                (* Character match.  Continue along the "true" path. *)
+                "t" <- "p"+8
+              } else {
+                (* Character non-match.  Continue along the "false" path. *)
+                "t" <- "p"+12
+              }
+            };;
+
+            "p" <-* "t"
+          } else {
+            Assert [Al b, Al t,
+              PRE[V] V "t" =*> V "p" * tree' b t (V "p")
+                * V "key" =?>8 wordToNat (V "keyLen") * mallocHeap 0
+              POST[_] Ex p, Ex t', V "t" =*> p * tree' (b %+ V "value") t' p
+                * V "key" =?>8 wordToNat (V "keyLen") * mallocHeap 0];;
+
+            (* The current position-character pair is not represented in the tree.  Let's add it here. *)
+            "c" <-- Call "malloc"!"malloc"(0, 4)
+            [Al b, Al t,
+              PRE[V, R] R =?> 4 * [| R <> 0 |] * V "t" =*> V "p" * tree' b t (V "p")
+                * V "key" =?>8 wordToNat (V "keyLen") * mallocHeap 0
+              POST[_] Ex p, Ex t', V "t" =*> p * tree' (b %+ V "value") t' p
+                * V "key" =?>8 wordToNat (V "keyLen") * mallocHeap 0];;
+
+            If ("c2" = 0) {
+              (* Informal invariant violated!  Key contains an internal '0' character. *)
+              Call "sys"!"abort"()
+              [PREonly[_] [| False |] ];;
+              Fail
+            } else {
+              Skip
+            };;
+
+            "c" *<- "pos";;
+            "c"+4 *<- "c2";;
+            "c"+8 *<- 0;;
+            "c"+12 *<- "p";;
+
+            "t" *<- "c";;
+            "t" <- "c"+8;;
+            "p" <- 0;;
+            "pos" <- "pos" + 1
+          }
+        } else {
+          (* We are ready to insert the final check, on string length. *)
+
+          "pos" <-- Call "malloc"!"malloc"(0, 4)
+          [Al b, Al t,
+            PRE[V, R] R =?> 4 * [| R <> 0 |] * V "t" =*> V "p" * tree' b t (V "p")
+            POST[_] Ex p, Ex t', V "t" =*> p * tree' (b %+ V "value") t' p];;
+
+          "pos" *<- "keyLen";;
+          "pos"+4 *<- 0;;
+          "pos"+8 *<- "value";;
+          "pos"+12 *<- "p";;
+
+          "t" *<- "pos";;
+          Return 0
+        }
+      }
     end
   }}.
 
@@ -212,16 +347,18 @@ Hint Extern 1 (@eq W _ _) => words.
 Ltac finish :=
   repeat match goal with
            | [ H : _ = _ |- _ ] => rewrite H
-         end; try rewrite natToW_wordToNat; auto.
-
-Ltac t' := sep hints; finish.
+         end; try rewrite natToW_wordToNat;
+  try apply tree'_weaken; auto.
 
 Ltac t :=
-  try match goal with
-        | [ |- context[debufferize] ] => unfold buffer
-      end;
-  try solve [ t' ];
-    post; evaluate hints; descend; try match_locals; t'.
+  match goal with
+    | [ |- forall stn_st specs, interp specs (Ex st', _ /\ [| evalInstrs _ _ (Assign (LvMem (Sp + natToW 0)%loc) (RvLval (LvReg Rp)) :: nil) = _ |])%PropX -> interp specs _ ] => solve [ sep hints ]
+    | _ =>
+      try match goal with
+            | [ |- context[debufferize] ] => unfold buffer
+          end;
+      post; evaluate hints; try (discriminate || tauto); descend; try match_locals; sep hints; finish
+  end.
 
 Theorem ok : moduleOk m.
   vcgen; abstract t.
